Equivalence.v
@@ -1,0 +1,38 @@
+Require Import Terms.
+
+Fixpoint rename_v (v:var) (r:Croot) : Croot :=
+match r with
+| Croot_exp e => Croot_exp (rename_exp_v v e)
+end
+with rename_exp_v (v:var) (e:Cexp) : Cexp :=
+match e with
+| Cexp_cont t          => Cexp_cont (rename_triv_v v t)
+| Cexp_app t0 t1 v' e' => let t0' := rename_triv_v v t0 in
+                          let t1' := rename_triv_v v t1 in
+                          Cexp_app t0' t1' v (rename_exp_v v e')
+end
+with rename_triv_v (v:var) (t:Ctriv) : Ctriv :=
+match t with
+| Ctriv_var x   => Ctriv_var x
+| Ctriv_lam x r => Ctriv_lam x (rename_v v r)
+| Ctriv_vvar _  => Ctriv_vvar v
+end.
+
+Definition a_eq (r1:Croot) (r2:Croot) := rename_v 0 r1 = rename_v 0 r2.
+Definition a_exp_eq (e1:Cexp) (e2:Cexp) := rename_exp_v 0 e1 = rename_exp_v 0 e2.
+Definition a_triv_eq (t1:Ctriv) (t2:Ctriv) :=
+  rename_triv_v 0 t1 = rename_triv_v 0 t2.
+
+Lemma rename_exp_v_inv :
+  forall (v v':var) (e:Cexp), rename_exp_v v (rename_exp_v v' e) = rename_exp_v v e.
+Proof.
+intros v v'.
+apply (Cexp_mut (fun r => rename_v v (rename_v v' r) = rename_v v r)
+                (fun t => rename_triv_v v (rename_triv_v v' t) = rename_triv_v v t)
+                (fun e => rename_exp_v v (rename_exp_v v' e) = rename_exp_v v e));
+intros; simpl; eauto.
+rewrite H; auto.
+rewrite H; auto.
+rewrite H; auto.
+rewrite H; rewrite H0; rewrite H1; auto.
+Qed.
