Terms.v
@@ -1,0 +1,53 @@
+Definition var := nat.
+
+Inductive Croot : Set :=
+| Croot_exp : Cexp -> Croot
+with Cexp : Set :=
+| Cexp_cont : Ctriv -> Cexp
+| Cexp_app  : Ctriv -> Ctriv -> var -> Cexp -> Cexp
+with Ctriv : Set :=
+| Ctriv_var : var -> Ctriv
+| Ctriv_vvar : var -> Ctriv
+| Ctriv_lam : var -> Croot -> Ctriv.
+
+Inductive CrootValid : Croot -> Prop :=
+| CrootValid_exp : forall e:Cexp, CexpValid e nil -> CrootValid (Croot_exp e)
+with CexpValid : Cexp -> list var -> Prop :=
+| CexpValid_cont : forall (ksi:list var) (t:Ctriv), CtrivValid t ksi nil -> CexpValid (Cexp_cont t) ksi
+| CexpValid_app  : forall (ksi0 ksi1 ksi2:list var) (t0 t1:Ctriv) (v:var) (e:Cexp),
+                     CtrivValid t1 ksi0 ksi1 -> CtrivValid t0 ksi1 ksi2 ->
+                     CexpValid e (v::ksi2) ->
+                     CexpValid (Cexp_app t0 t1 v e) ksi0
+with CtrivValid : Ctriv -> list var -> list var -> Prop :=
+| CtrivValid_vvar : forall (ksi:list var) (v:var), CtrivValid (Ctriv_vvar v) (v::ksi) ksi
+| CtrivValid_var  : forall (ksi:list var) (x:var), CtrivValid (Ctriv_var x) ksi ksi
+| CtrivValid_lam  : forall (ksi:list var) (x:var) (r:Croot), CrootValid r -> CtrivValid (Ctriv_lam x r) ksi ksi.
+
+Scheme Croot_mut := Induction for Croot Sort Type
+with Ctriv_mut := Induction for Ctriv Sort Type
+with Cexp_mut := Induction for Cexp Sort Type.
+
+Scheme CrootValid_mut := Induction for CrootValid Sort Prop
+with CtrivValid_mut := Induction for CtrivValid Sort Prop
+with CexpValid_mut := Induction for CexpValid Sort Prop.
+
+Hint Constructors Ctriv Cexp Croot.
+Hint Constructors CtrivValid CexpValid CrootValid.
+
+Inductive Droot : Set :=
+| Droot_exp : Dexp -> Droot
+with Dexp : Set :=
+| Dexp_app  : Dexp -> Dexp -> Dexp
+| Dexp_triv : Dtriv -> Dexp
+with Dtriv : Set :=
+| Dtriv_var : var -> Dtriv
+| Dtriv_lam : var -> Droot -> Dtriv.
+
+Scheme Droot_mut := Induction for Droot Sort Type
+with Dexp_mut := Induction for Dexp Sort Type
+with Dtriv_mut := Induction for Dtriv Sort Type.
+
+Hint Constructors Droot Dexp Dtriv.
+
+Definition Cont := var -> Ctriv -> Cexp.
+
