Makefile
@@ -1,0 +1,15 @@
+MODULES := Terms Equivalence Inverse Transformations
+
+VS := $(MODULES:%=%.v)
+
+.PHONY: coq clean
+
+coq: Makefile.coq
+	$(MAKE) -j2 -f Makefile.coq
+
+Makefile.coq: Makefile $(VS)
+	coq_makefile $(VS) -o Makefile.coq
+
+clean:: Makefile.coq
+	$(MAKE) -f Makefile.coq clean
+	rm -f Makefile.coq
